Add fermat_inv_pe to DGK impl

code/experimental/he/Hacl.Impl.HE.DGK.fst
@@ -248,7 +248,7 @@ let check_is_zero #nLen sk c =
   pop_frame ();
   b
 
-val carm_pe:
+val carm_pe_impl:
      #nLen:bn_len_s
   -> p:lbignum nLen
   -> e:lbignum nLen
@@ -259,13 +259,17 @@ val carm_pe:
       disjoint p res /\ disjoint e res /\
       isprm (as_snat h p) /\
       as_snat h e > 0 /\
-      nat_fits (as_snat h e) nLen /\
       nat_fits (exp (as_snat h p) (as_snat h e)) nLen)
      (ensures fun h0 _ h1 ->
       modifies1 res h0 h1 /\
       as_snat h1 res = carm_pe (as_snat h0 p) (as_snat h0 e))
-let carm_pe #nLen p e res =
+let carm_pe_impl #nLen p e res =
+  let hp0 = FStar.HyperStack.ST.get () in
   bn_len_s_fits nLen;
+  exp_greater_than_power (as_snat hp0 p) (as_snat hp0 e);
+  nat_fits_trans (as_snat hp0 e)
+                 (exp (as_snat hp0 p) (as_snat hp0 e))
+                 nLen;
 
   push_frame ();
 
@@ -283,7 +287,47 @@ let carm_pe #nLen p e res =
 
   bn_exp p e res;
   bn_exp p e' tmp;
-
   bn_sub_exact res tmp res;
+
+  pop_frame ()
+
+val fermat_inv_pe:
+     #nLen:bn_len_s
+  -> p:lbignum nLen
+  -> e:lbignum nLen
+  -> a:lbignum nLen
+  -> res:lbignum nLen
+  -> Stack unit
+    (requires fun h ->
+      live h p /\ live h e /\ live h a /\ live h res /\
+      disjoint p res /\ disjoint a res /\ disjoint e res /\
+      isprm (as_snat h p) /\
+      as_snat h e > 0 /\
+      as_snat h a < exp (as_snat h p) (as_snat h e) /\
+      nat_fits (exp (as_snat h p) (as_snat h e)) nLen)
+    (ensures fun h0 _ h1 ->
+      modifies1 res h0 h1 /\
+      as_snat h1 res =
+        S.fermat_inv_pe (as_snat h0 p) (as_snat h0 e) (as_snat h0 a))
+let fermat_inv_pe #nLen p e a res =
+  bn_len_s_fits nLen;
+  push_frame ();
+
+  let lam = create nLen (u64 0) in
+  carm_pe_impl p e lam;
+
+  let one:lbignum 1ul = bn_one #1ul in
+  bn_sub_exact lam one lam;
+
+  let hp = FStar.HyperStack.ST.get () in
+  assert (as_snat hp lam = carm_pe (as_snat hp p) (as_snat hp e) - 1);
+
+  let m = bn_copy p in
+  bn_exp m e res; copy m res;
+
+  bn_modular_exp m a lam res;
+
+  let hp = FStar.HyperStack.ST.get () in
+  to_fe_idemp #(as_snat hp m) (as_snat hp a);
 
   pop_frame ()
